$$
y'=f(x)g(y)
$$
$$
M(x)N(y)dx+P(x)Q(y)dy=0
$$
$$
x^{2}y^{2}y'+1=y
$$
$$
x^{2}y^{2}\tfrac{dx}{dy}=y-1
$$
$$
x^{2}y^{2}dy=(y-1)dx
$$

$$
y''+y'-2y=0
$$
$$
y''-2y'-3y=e^{4x}
$$
$$
y''-9y=e^{3x}\cos(x)
$$

$$
\begin{cases}
    \dot{x}=y+2e^t \\
    \dot{y}=x+t^2
\end{cases}
$$
$$
\begin{cases}
    \ddot{x}=2x-4y \\
    \ddot{y}=x-3y+3e^t
\end{cases}
$$

$$
\dot{x}=Ax, \\
A=
\begin{pmatrix}
    2 & -1 & -1  \\ 
    1 & 0 & -1  \\ 
    3 & -2 & -2
\end{pmatrix}
$$
$$
\dot{x}=Ax, \\
A=
\begin{pmatrix}
    1 & -2\\
    2 & -3 
\end{pmatrix}
$$